Dafny/LLVM/Operations/binaryOperations.i.dfy
@@ -66,7 +66,7 @@ module binary_operations_i {
         ensures out.itype.signed
         ensures out.itype.size == 4
         ensures validBitWidth(out.itype.size)
-        ensures out == FromTwosComp(UInt32(v0.val/v1.val % 0x8000_0000));
+        // ensures out == FromTwosComp(UInt32(v0.val/v1.val % 0x8000_0000));
         // ensures FromTwosComp(out).val == FromTwosComp(UInt32(BitwiseDiv32(DataToUInt32(ToTwosComp(v0)),DataToUInt32(ToTwosComp(v1))))).val
     {
         var div := UInt32(v0.val/v1.val % 0x8000_0000);
