Dafny/examples/Challenge8/Challenge8PropertiesNEW.i.dfy
@@ -19,19 +19,61 @@ module challenge8Properties{
     import opened binary_operations_i
     import opened ops
 
-    lemma vulnRefactor(s:State,c:seq<Code>) returns (preB:Behavior)
+
+    lemma returnBlockNoStutter(s:State) returns (b:Behavior)
+        requires ValidState(s);
+        requires validIntState(s);
+        requires validConfig(s);
+    {
+        var config := allVariablesConfig();
+
+        b := [s] + evalCodeFn(return_(),s);
+        assert NextStep(b[0],b[1],evalInsStep((LOAD(config.ops["var_26"],1,config.ops["var_retval"]))));
+        assert NextStep(b[1],b[2],evalInsStep((RET(config.ops["var_26"]))));
+        assert |b| == 3;
+        assert ValidBehavior(b);
+    }
+
+    lemma ifThen19NoStutter(s:State) returns (b:Behavior)
+        requires ValidState(s);
+        requires validIntState(s);
+        requires validConfig(s);
+        ensures b == [s] + evalCodeFn(if_then19(),s);
+        ensures |b| == 5;
+        ensures NextStep(b[0],b[1],evalInsStep((CALL(D(Void),delete_connection()))));
+        ensures NextStep(b[1],b[2],evalInsStep((STORE(D(Int(0,IntType(1,false))),allVariablesConfig().ops["var_retval"]))));
+        ensures NextStep(b[2],b[3],evalInsStep((LOAD(allVariablesConfig().ops["var_26"],1,allVariablesConfig().ops["var_retval"]))));
+        ensures NextStep(b[3],b[4],evalInsStep((RET(allVariablesConfig().ops["var_26"]))));
+
+{
+    var config := allVariablesConfig();
+    b := [s] + evalCodeFn(if_then19(),s);
+    assert |b| == 5;
+    assert NextStep(b[0],b[1],evalInsStep((CALL(D(Void),delete_connection()))));
+
+    assert NextStep(b[1],b[2],evalInsStep((STORE(D(Int(0,IntType(1,false))),config.ops["var_retval"]))));
+    var rB := returnBlockNoStutter(b[2]);
+}
+
+
+
+
+
+
+// Eval using Stutter Step // 
+        lemma vulnRefactor(s:State,c:seq<Code>) returns (preB:Behavior)
         requires ValidState(s);
         requires validStartingState(s);
         requires c == challenge_8_transport_handler_create_conn_vuln_test();
         ensures ValidBehavior(preB);
         ensures |preB| == 8;
         ensures forall i :: i >=0 && i < |preB| - 1 ==> NextStep(preB[i],preB[i+1],Step.stutterStep());
-        ensures preB == [s] + evalCodeSeqFn(c,s);
+        ensures preB == [s] + evalCodeSeqFn_Stutter(c,s);
     {
         //    [prefixCode(), Block([CNil]),postfixCode()]
 
         reveal_ValidBehavior();
-        var b:Behavior := [s] + evalCodeSeqFn(c,s);
+        var b:Behavior := [s] + evalCodeSeqFn_Stutter(c,s);
         assert |b| == 8;
         assert ValidBehavior(b);
         forall i | i >=0 && i < |b| - 1
@@ -40,15 +82,15 @@ module challenge8Properties{
             // assert NextStep(b[i],b[i+1],Step.stutterStep());
         }
 
-        var prefixB :=  [s] + evalCodeFn(prefixCode(),s);
+        var prefixB :=  [s] + evalCodeFn_Stutter(prefixCode(),s);
         assert |prefixB| == 3;
         assert prefixB == b[..3];
 
-        var midB :=  evalCodeFn(Block([CNil]),last(prefixB));
+        var midB :=  evalCodeFn_Stutter(Block([CNil]),last(prefixB));
         assert |midB| == 2;
         assert midB == b[3..5];
 
-        var postfixB :=  evalCodeFn(postfixCode(),last(midB));
+        var postfixB :=  evalCodeFn_Stutter(postfixCode(),last(midB));
         assert |postfixB| == 2;
 
         assert b == prefixB + midB + postfixB + [last(postfixB)];
@@ -57,75 +99,8 @@ module challenge8Properties{
 
     }
 
-    lemma patchRefactor(s:State,c:seq<Code>,size:Operand) returns (postB:Behavior)
-        requires ValidState(s);
-        requires validStartingState(s);
-        requires size.D?;
-        requires size.d.Int?;
-        requires size.d.itype == IntType(4,false);
-        requires ValidOperand(s,size)
-        requires c == challenge_8_transport_handler_create_conn_patch(size);
-        requires validConfig(s);
-
-        ensures postB ==  [s] + evalCodeSeqFn(c,s);
-    {
-        reveal_ValidBehavior();
-        var config := allVariablesConfig();    
-        postB := [s] + evalCodeSeqFn(c,s);
-        // assert postB == [s] + evalCodeSeqFn(c,s)
-        var prefixB :=  [s] + evalCodeFn(prefixCode(),s);
-        var mid := evalCodeFn(patch_block(size),last(prefixB));
-        var post := evalCodeFn(postfixCode(),last(mid));
-        assert all_but_last(prefixB) == postB[..2];
-        // assert all_but_last(mid) ==  postB[2..2+|mid|];
-        // assert postB == all_but_last(prefixB) +  all_but_last(mid) + post;
-        // assert |prefixB| == 3;
-        // var vulnB := vulnRefactor(s,challenge_8_transport_handler_create_conn_vuln_test());
-        // var vb:Behavior := [s] + evalCodeSeqFn(challenge_8_transport_handler_create_conn_vuln_test(),s);
-        // assert prefixB == vulnB[..3];
-        // assert prefixB == postB[..3];
-        
-        // assert s == postB[1] == postB[2] == postB[0];
-        assert NextStep(postB[0],postB[1],Step.stutterStep());
-        assert NextStep(postB[1],postB[2],Step.stutterStep());
-
-        // assert (config.ops["var_div"].LV? || config.ops["var_div"].GV?)  
-        //         && ValidOperand(postB[2],config.ops["var_div"]) && ValidOperand(s,size) 
-        //         && ValidOperand(postB[2],D(Int(7,IntType(4,false))));
-        // assert isInt(OperandContents(postB[2],size)); 
-        // assert typesMatch(OperandContents(postB[2],size),OperandContents(postB[2],D(Int(7,IntType(4,false)))));
-        assert ValidState(postB[2]);
-        assert ValidInstruction(postB[2], (SDIV(config.ops["var_div"],size,D(Int(7,IntType(4,false))))));
-        var s'' := stateUpdateVar(postB[2],config.ops["var_div"],evalSDIV(OperandContents(postB[2],size),OperandContents(postB[2],D(Int(7,IntType(4,false))))));
-        s'' :=  incPC(s'');
-        assert ValidData(s'',evalSDIV(OperandContents(postB[2],size),OperandContents(postB[2],D(Int(7,IntType(4,false))))));
-        assert s''.ok;
-        assert patch_block(size).block[0] == Ins(SDIV(config.ops["var_div"],size,D(Int(7,IntType(4,false)))));
-        assert ValidState(s'');
-        assert  config.ops["var_div"].LV?;
-        assert s''.pc == postB[2].pc +1;
-        assert s'' == postB[2].(lvs := postB[2].lvs[config.ops["var_div"].l := evalSDIV(OperandContents(postB[2],size),OperandContents(postB[2],D(Int(7,IntType(4,false)))))],o := Nil,pc := postB[2].pc +1); 
-        // assert evalUpdate(postB[2], config.ops["var_div"], evalSDIV(OperandContents(postB[2],size),OperandContents(postB[2],D(Int(7,IntType(4,false))))),s'');
-        // assert postB[3] == evalInsRe((SDIV(config.ops["var_div"],size,D(Int(7,IntType(4,false))))),post[2]);
-        assert validEvalIns((SDIV(config.ops["var_div"],size,D(Int(7,IntType(4,false))))),postB[2],s'');
-
-        // assert ValidState(x);
-        assert NextStep(postB[2],postB[3],evalInsStep((SDIV(config.ops["var_div"],size,D(Int(7,IntType(4,false)))))));
-        // assert ValidState(postB[3]);
-        // assert NextStep(postB[3],postB[4],evalInsStep((ICMP(config.ops["var_cmp17"],sgt,4,config.ops["var_num_packets"],config.ops["var_div"]))));
-        // if dataToBool(OperandContents(postB[4],config.ops["var_cmp17"])){
-        // //     assert NextStep(postB[4],postB[5],evalInsStep((CALL(D(Void),delete_connection()))));
-        // }else{
-        // //     assert NextStep(postB[4],postB[5],Step.stutterStep());
-        // }
-        // assert NextStep(postB[4],postB[5],evalInsStep((ICMP(config.ops["var_cmp17"],sgt,4,config.ops["var_num_packets"],config.ops["var_div"]))));
-
-
-        // assert vb
-    }
-
     lemma behaviorIsSumOfParts(s:State,cseq:seq<Code>,b:Behavior)
-        requires b == [s] + evalCodeSeqFn(cseq,s)
+        requires b == [s] + evalCodeSeqFn_Stutter(cseq,s)
         requires |cseq| > 1;
     {
         var smalB := b;
@@ -133,32 +108,33 @@ module challenge8Properties{
         smalB := smalB[1..];
         // var index := 1;
         var i := 0;
-        var subB := evalCodeFn(cseq[i],s);
+        var subB := evalCodeFn_Stutter(cseq[i],s);
         assert smalB[..|subB|] == subB;
         
         smalB := smalB[|subB|..];
 
-        assert evalCodeSeqFn(cseq,s) == evalCodeFn(first(cseq),s) + evalCodeSeqFn(all_but_first(cseq),last(evalCodeFn(first(cseq),s)));
-        assert subB ==  evalCodeFn(first(cseq),s);
-        // assert evalCodeSeqFn(all_but_first(cseq),last(evalCodeFn(first(cseq),s))) == evalCodeFn(first(all_but_first(cseq)),last(evalCodeFn(first(cseq),s)))
+        assert evalCodeSeqFn_Stutter(cseq,s) == evalCodeFn_Stutter(first(cseq),s) + evalCodeSeqFn_Stutter(all_but_first(cseq),last(evalCodeFn_Stutter(first(cseq),s)));
+        assert subB ==  evalCodeFn_Stutter(first(cseq),s);
+        // assert evalCodeSeqFn_Stutter(all_but_first(cseq),last(evalCodeFn_Stutter(first(cseq),s))) == evalCodeFn_Stutter(first(all_but_first(cseq)),last(evalCodeFn_Stutter(first(cseq),s)))
         // index := 1+|subB|;
         // i := i +1;
-        // subB := evalCodeFn(cseq[i],last(subB));
+        // subB := evalCodeFn_Stutter(cseq[i],last(subB));
         // assert b[..|subB|] == subB;
         // while i < |cseq|
         // {
-        //     var subB := evalCodeFn(cseq[i],b[index-1]);
+        //     var subB := evalCodeFn_Stutter(cseq[i],b[index-1]);
         //     assert b[index..index+|subB|] == subB;
         //     index := index+|subB|;
         //     i := i +1;
         // }
     //    forall i | i >= 0 && i < |cseq|
     //    {
-    //      var subB := evalCodeFn(prefixCode(),b[index-1]);
+    //      var subB := evalCodeFn_Stutter(prefixCode(),b[index-1]);
     //      assert b[index..index+|subB|] == subB;
     //      index := index+|subB|;
     //    }
     }
+
 
     lemma fullPatch(s:State,size:Operand)returns (b:Behavior)
         requires ValidState(s);
@@ -168,13 +144,13 @@ module challenge8Properties{
         requires size.d.itype == IntType(4,false);
         requires ValidOperand(s,size)
         requires validConfig(s);
-        ensures b ==  [s] + evalCodeSeqFn(challenge_8_transport_handler_create_conn_patch(size),s);
+        ensures b ==  [s] + evalCodeSeqFn_Stutter(challenge_8_transport_handler_create_conn_patch(size),s);
     {
         var config := allVariablesConfig();    
-        b := [s] + evalCodeSeqFn(challenge_8_transport_handler_create_conn_patch(size),s);   
-        var prefixB :=  [s] + evalCodeFn(prefixCode(),s);
-        var mid := evalCodeFn(patch_block(size),last(prefixB));
-        // var post := evalCodeFn(postfixCode(),last(mid));
+        b := [s] + evalCodeSeqFn_Stutter(challenge_8_transport_handler_create_conn_patch(size),s);   
+        var prefixB :=  [s] + evalCodeFn_Stutter(prefixCode(),s);
+        var mid := evalCodeFn_Stutter(patch_block(size),last(prefixB));
+        // var post := evalCodeFn_Stutter(postfixCode(),last(mid));
 
         assert NextStep(b[0],b[1],Step.stutterStep());
         assert NextStep(b[1],b[2],Step.stutterStep());
@@ -197,16 +173,31 @@ module challenge8Properties{
         requires size.d.Int?;
         requires size.d.itype == IntType(4,false);
     {
-       assert forall s :: |evalCodeFn(postfixCodeSimple(),s)| == 4;
+       assert forall s :: |evalCodeFn_Stutter(postfixCodeSimple(),s)| == 4;
         var config := allVariablesConfig();
 
-       && b == [s] + evalCodeFn(patch_block(size),s)
+    //    && b == [s] + evalCodeFn_Stutter(patch_block(size),s)
+        // && ValidBehavior(b)
+       && ValidState(s)
+       && validStartingState(s)
        && |b| >= 8
-       && b[|b|-5..] == evalCodeFn(postfixCodeSimple(),b[|b|-6]) + [last(b)]
+       && b[|b|-5..] == evalCodeFn_Stutter(postfixCodeSimple(),b[|b|-6]) + [last(b)]
        && FromTwosComp(UInt32(size.d.val/Int(7,IntType(4,false)).val % 0x8000_0000)).val < (OperandContents(s,config.ops["var_num_packets"]).val)
     }
 
+    lemma vulnPostfixSimple(s:State,size:Operand) returns (b:Behavior)
+        requires ValidState(s);
+        requires validStartingState(s);
+        requires size.D?;
+        requires size.d.Int?;
+        requires size.d.itype == IntType(4,false);
+        requires ValidOperand(s,size)
+        requires validConfig(s);
+    {
+        var config := allVariablesConfig();
+        b := [s] + evalCodeSeqFn_Stutter(challenge_8_transport_handler_create_conn_vuln_postfix_simple(size),s);
 
+    }
     lemma patchBlock(s:State,size:Operand) returns (b:Behavior)
         requires ValidState(s);
         requires validStartingState(s);
@@ -215,30 +206,27 @@ module challenge8Properties{
         requires size.d.itype == IntType(4,false);
         requires ValidOperand(s,size)
         requires validConfig(s);
-        ensures b ==  [s] + evalCodeFn(patch_block(size),s);
+        ensures b ==  [s] + evalCodeFn_Stutter(patch_block(size),s);
         ensures |b| >= 8;
         ensures !miniSpec(s,b,size);
         // ensures ValidBehavior(b);
     {
         var config := allVariablesConfig();
-        b := [s] + evalCodeFn(patch_block(size),s);
+        b := [s] + evalCodeFn_Stutter(patch_block(size),s);
 
         assert NextStep(b[0],b[1],evalInsStep((SDIV(config.ops["var_div"],size,D(Int(7,IntType(4,false)))))));
         // assert ValidState(b[1]);
         assert NextStep(b[1],b[2],evalInsStep((ICMP(config.ops["var_cmp17"],sgt,4,config.ops["var_num_packets"],config.ops["var_div"]))));
         if dataToBool(OperandContents(b[2],config.ops["var_cmp17"])){
-            // assert evalCodeFn(c.ifTrue,s);
+            // assert evalCodeFn_Stutter(c.ifTrue,s);
             assert patch_block(size).block[2].IfElse?;
-            var ifElseB := evalCodeFn(patch_block(size).block[2].ifTrue,b[2]);
+            var ifElseB := evalCodeFn_Stutter(patch_block(size).block[2].ifTrue,b[2]);
             assert b == [s] + [b[1]] + [b[2]] + ifElseB + [last(ifElseB)];
             var ifThen19:Behavior := ifThen19(b[2]);
-            assert [b[2]] + evalCodeFn(patch_block(size).block[2].ifTrue,b[2]) == ifThen19; 
+            assert [b[2]] + evalCodeFn_Stutter(patch_block(size).block[2].ifTrue,b[2]) == ifThen19; 
             // assert b == [s] + [b[1]] + ifThen19 + [last(ifThen19)];
-
-                        // assert |ifElseB| == |ifThen19|;
-
-            assert b[2..2+|ifThen19|] == ifThen19;
-            assert b[2..] == ifThen19 + [last(ifThen19)];
+            // assert b[2..2+|ifThen19|] == ifThen19;
+            // assert b[2..] == ifThen19 + [last(ifThen19)];
             assert NextStep(b[2],b[3],evalInsStep((CALL(D(Void),delete_connection()))));
             assert NextStep(b[3],b[4],evalInsStep((STORE(D(Int(0,IntType(1,false))),allVariablesConfig().ops["var_retval"]))));
             assert NextStep(b[4],b[5],evalInsStep((LOAD(allVariablesConfig().ops["var_26"],1,allVariablesConfig().ops["var_retval"]))));
@@ -273,7 +261,7 @@ module challenge8Properties{
         requires ValidState(s);
         requires validIntState(s);
         requires validConfig(s);
-        ensures b == [s] + evalCodeFn(return_(),s);
+        ensures b == [s] + evalCodeFn_Stutter(return_(),s);
         ensures |b| == 4;
         ensures NextStep(b[0],b[1],evalInsStep((LOAD(allVariablesConfig().ops["var_26"],1,allVariablesConfig().ops["var_retval"]))));
         ensures NextStep(b[1],b[2],evalInsStep((RET(allVariablesConfig().ops["var_26"]))));
@@ -281,7 +269,7 @@ module challenge8Properties{
     {
     var config := allVariablesConfig();
 
-    b := [s] + evalCodeFn(return_(),s);
+    b := [s] + evalCodeFn_Stutter(return_(),s);
     assert StateNext(b[0],b[1]);
     assert ValidState(b[1]);
     assert ValidState(b[2]);
@@ -290,14 +278,13 @@ module challenge8Properties{
     assert NextStep(b[0],b[1],evalInsStep((LOAD(config.ops["var_26"],1,config.ops["var_retval"]))));
     assert NextStep(b[1],b[2],evalInsStep((RET(config.ops["var_26"]))));
     assert NextStep(b[2],b[3],Step.stutterStep());
-
 }
 
 lemma ifThen19(s:State) returns (b:Behavior)
     requires ValidState(s);
     requires validIntState(s);
     requires validConfig(s);
-    ensures b == [s] + evalCodeFn(if_then19(),s);
+    ensures b == [s] + evalCodeFn_Stutter(if_then19(),s);
     ensures |b| == 7;
     ensures NextStep(b[0],b[1],evalInsStep((CALL(D(Void),delete_connection()))));
     ensures NextStep(b[1],b[2],evalInsStep((STORE(D(Int(0,IntType(1,false))),allVariablesConfig().ops["var_retval"]))));
@@ -309,7 +296,7 @@ lemma ifThen19(s:State) returns (b:Behavior)
 {
     var config := allVariablesConfig();
 
-    b := [s] + evalCodeFn(if_then19(),s);
+    b := [s] + evalCodeFn_Stutter(if_then19(),s);
     assert |b| == 7;
     assert NextStep(b[0],b[1],evalInsStep((CALL(D(Void),delete_connection()))));
     // assert  ValidState(b[1]);
@@ -330,6 +317,9 @@ lemma ifThen19(s:State) returns (b:Behavior)
     assert NextStep(b[5],b[6],Step.stutterStep());
 }
 
+/// VV OLD  VV /// 
+
+
 // lemma
 
 
@@ -341,13 +331,13 @@ lemma ifThen19(s:State) returns (b:Behavior)
 //     {
 //         reveal_ValidBehavior();
 //         //    [ Block([CNil]), Block([CNil]), Block([CNil])]
-//         var b:Behavior := evalCodeSeqFn(c,s);
+//         var b:Behavior := evalCodeSeqFn_Stutter(c,s);
 //         assert ValidSimpleBehavior([s] + b);
 //         assert |b| >= 0;
 //         assert c == [ Block([CNil]), Block([CNil]), Block([CNil])];
 
 //         var step,remainder,subB := unwrapCodeWitness(b,c,s);
-//         assert step == evalCodeFn(Block([CNil]),s);
+//         assert step == evalCodeFn_Stutter(Block([CNil]),s);
 //         assert remainder == [Block([CNil]), Block([CNil])];
 //         // lets dive into the block
 //             var subStep,subRemainder,subSubB := unwrapCodeWitness(step,[CNil],s);
@@ -360,7 +350,7 @@ lemma ifThen19(s:State) returns (b:Behavior)
 
 //         var s' := last(step);
 //         step,remainder,subB := unwrapCodeWitness(subB,remainder,s');
-//         assert step == evalCodeFn(Block([CNil]),s');
+//         assert step == evalCodeFn_Stutter(Block([CNil]),s');
 //         assert remainder == [ Block([CNil])];
 //             // lets dive into the block
 //             subStep,subRemainder,subSubB := unwrapCodeWitness(step,[CNil],s');
@@ -373,7 +363,7 @@ lemma ifThen19(s:State) returns (b:Behavior)
 
 //         s' := last(step);
 //         step,remainder,subB := unwrapCodeWitness(subB,remainder,s');
-//         assert step == evalCodeFn(Block([CNil]),s');
+//         assert step == evalCodeFn_Stutter(Block([CNil]),s');
 //         assert remainder == [];
 
 //         assert subB == [s'];
@@ -396,12 +386,12 @@ lemma ifThen19(s:State) returns (b:Behavior)
 //     {
 //         reveal_ValidBehavior();
 //         //    [ Block([CNil]), Block([CNil]), Block([CNil])]
-//         // var b:Behavior := evalCodeSeqFn(c,s);
+//         // var b:Behavior := evalCodeSeqFn_Stutter(c,s);
 //         // assert ValidSimpleBehavior([s] + b);
 //         // assert |b| >= 0;
         
 //         // var step,remainder,subB := unwrapCodeWitness(b,c,s);
-//         // assert step == evalCodeFn(Block([CNil]),s);
+//         // assert step == evalCodeFn_Stutter(Block([CNil]),s);
 //         // // assert remainder == [patch_block,postfixCode()];
 //         // // lets dive into the block
 //         //     var subStep,subRemainder,subSubB := unwrapCodeWitness(step,[CNil],s);
@@ -418,11 +408,11 @@ lemma ifThen19(s:State) returns (b:Behavior)
 //         // step,remainder,subB := unwrapCodeWitness(subB,remainder,s');
 //         // assert remainder == [ Block([CNil])];
 //         //  // lets dive into the block
-//         //     assert step == evalCodeFn(first(mainBlock),s');
+//         //     assert step == evalCodeFn_Stutter(first(mainBlock),s');
 //         //     assert first(mainBlock).Block?;
-//         //     assert step == evalCodeSeqFn(first(mainBlock).block,s');
+//         //     assert step == evalCodeSeqFn_Stutter(first(mainBlock).block,s');
 
-//         //     // assert step == evalCodeSeqFn(first(mainBlock),s');
+//         //     // assert step == evalCodeSeqFn_Stutter(first(mainBlock),s');
 //         //     subStep,subRemainder,subSubB := unwrapCodeWitness(step,first(mainBlock).block,s');
 //         //     assert |subStep| == 1;
 //         //     assert s'.ok;
@@ -453,7 +443,7 @@ lemma ifThen19(s:State) returns (b:Behavior)
 //         //     subStep,subRemainder,subSubB := unwrapCodeWitness(subSubB,subRemainder,s');
              
 //         //         if dataToBool(OperandContents(s',first(nextIns).ifCond)){
-//         //             assert subStep == evalCodeFn(first(nextIns).ifTrue,s');
+//         //             assert subStep == evalCodeFn_Stutter(first(nextIns).ifTrue,s');
 //         //             // new block that needs unwrapping 
 //         //             patchBehavorsTestsubBlock(subStep,first(nextIns).ifTrue,s');
 //         //             // var if_true_block := first(nextIns).ifTrue;
@@ -472,7 +462,7 @@ lemma ifThen19(s:State) returns (b:Behavior)
 
 
 //         //         }else{
-//         //             assert subStep == evalCodeFn(first(nextIns).ifFalse,s');
+//         //             assert subStep == evalCodeFn_Stutter(first(nextIns).ifFalse,s');
 //         //             assert subRemainder == [];
 //         //             assert subSubB == [s']; 
 //         //             assert b[4] == subStep[0]; 
@@ -482,7 +472,7 @@ lemma ifThen19(s:State) returns (b:Behavior)
         
 //         // s' := last(step);
 //         // step,remainder,subB := unwrapCodeWitness(subB,remainder,s');
-//         // assert step == evalCodeFn(Block([CNil]),s');
+//         // assert step == evalCodeFn_Stutter(Block([CNil]),s');
 //         // assert remainder == [];
 
 //         // assert subB == [s'];
@@ -494,13 +484,13 @@ lemma ifThen19(s:State) returns (b:Behavior)
 //         requires c == if_then19();
 //         requires ValidState(s);
 //         requires validConfig(s,allVariablesConfig());
-//         requires b == evalCodeSeqFn(c.block,s);
+//         requires b == evalCodeSeqFn_Stutter(c.block,s);
 //         ensures  first(c.block).Ins?;
 //         ensures first(c.block).ins.CALL?;
         
         
 //     {
-//         var Behavior := evalCodeSeqFn(c.block,s);
+//         var Behavior := evalCodeSeqFn_Stutter(c.block,s);
 //         var initalCode := c.block;
 //         var step,remainder,subB := unwrapCodeWitness(b,c.block,s);
 //         assert |step| == 1;
